Adding requirement that the nodes of the factor graph be consecutive natural numbers starting from 0, fixing issue where we assumed that every function in the function map was a probability function rather than only those that correspond to valid functions, improving comments, functions for adding variable nodes to the factor graph, helper theorems to prove things about the disjoint sum version of the count set, function for adding a function node to the factor graph, template for proof of well-formedness of the addition of variable nodes and function nodes, proving lemma (we can swap the order of the two elements in a two-element set), proved lemma (we can swap the order of the inputs to the function which adds an edge), added function for adding an edge, function for adding several variable and function nodes at once

ConvolutionalCodes/factor_graphScript.sml
@@ -3,6 +3,7 @@ open HolKernel Parse boolLib bossLib;
 open probabilityTheory;
 (*open listTheory;*)
 open fsgraphTheory;
+open pred_setTheory;
 
 val _ = new_theory "factor_graphs";
 
@@ -65,6 +66,9 @@ val _ = new_theory "factor_graphs";
 (*                                                                            *)
 (* We restrict our attention to factor graphs with binary inputs and outputs  *)
 (* which represent probabilities (of type extreal).                           *)
+(*                                                                            *)
+(* We expect the nodes of the factor graph to be consecutive natural numbers  *)
+(* starting from 0.                                                           *)
 (* -------------------------------------------------------------------------- *)
 Datatype:
   factor_graph =
@@ -85,6 +89,7 @@ End
 (*   0 and 1                                                                  *)
 (* - the variables used as input to each function must be amongst the         *)
 (*   variable_nodes.                                                          *)
+(* - the nodes should be the consecutive natural numbers starting from 0      *)
 (* - We currently don't require that the input to the function map itself has *)
 (*   to be a function node, because this doesn't gel well with the            *)
 (*   representation of functions in HOL, which requires a function to have a  *)
@@ -99,10 +104,12 @@ Definition wffactor_graph_def:
   (gen_bipartite fg.underlying_graph fg.function_nodes fg.variable_nodes)
   ) ∧
   (∀f bs.
-     let
-       output = (SND (fg.function_map f)) bs;
+     f ∈ fg.function_nodes ⇒
+     (let
+        output = (SND (fg.function_map f)) bs;
      in
        0 ≤ output ∧ output ≤ 1
+     )
   ) ∧
   (∀f.
      f ∈ fg.function_nodes ⇒
@@ -111,6 +118,9 @@ Definition wffactor_graph_def:
      in
        ∀x. x ∈ (set variables) ⇒ x ∈ fg.variable_nodes
      )
+  ) ∧
+  (∃n.
+     fg.variable_nodes ∪ fg.function_nodes = {INR i | i ∈ count n}
   )
   )
 End
@@ -130,33 +140,245 @@ End
 (* -------------------------------------------------------------------------- *)
 (* The empty graph is bipartite into the empty set and the empty set          *)
 (*                                                                            *)
-(* This theorem would be convenient, but isn't true, becuase                  *)
-(*                                                                            *)
+(* This theorem would be convenient, but isn't true, because a partition is   *)
+(* only considered to be valid if each of the components is nonempty. I don't *)
+(* think this should be how a partition is defined, but on the other hand,    *)
+(* there is some precedent for this.                                          *)
 (* -------------------------------------------------------------------------- *)
 (*Theorem gen_bipartite_empty[simp]:
   gen_bipartite emptyG ∅ ∅
 Proof
   gvs[gen_bipartite_def]
 QED*)
-
+ 
 (* -------------------------------------------------------------------------- *)
 (* Prove that the empty factor graph is well-formed                           *)
 (* -------------------------------------------------------------------------- *)
-Theorem fg_empty_wf:
+Theorem fg_empty_wf[simp]:
   wffactor_graph fg_empty
 Proof
   gvs[fg_empty_def, wffactor_graph_def]
-  >> rpt strip_tac
+  >- (qexists ‘0’ >> gvs[])
 QED
 
 (* -------------------------------------------------------------------------- *)
+(* Add a variable node to the factor_graph.                                   *)
 (*                                                                            *)
-(*                                                                            *)
-(*                                                                            *)
+(* The first node added (variable or function) should be 0, the next node     *)
+(* should be 1, etc.                                                          *)
 (* -------------------------------------------------------------------------- *)
-Definition factor_graph_add_node_def:
-  factor_graph_add_node fg node = 
+Definition fg_add_variable_node_def:
+  fg_add_variable_node fg =
+  let
+    new_node = (INR (CARD (nodes fg.underlying_graph)))
+  in
+    fg with
+       <|
+         underlying_graph := fsgAddNode new_node fg.underlying_graph;
+         variable_nodes := new_node INSERT fg.variable_nodes
+       |>
 End
+
+(* -------------------------------------------------------------------------- *)
+(* Adds n variable nodes to the factor graph                                  *)
+(* -------------------------------------------------------------------------- *)
+Definition fg_add_n_variable_nodes_def:
+  fg_add_n_variable_nodes fg 0 = fg ∧
+  fg_add_n_variable_nodes fg (SUC n) =
+  fg_add_variable_node (fg_add_n_variable_nodes fg)
+End
+
+(* -------------------------------------------------------------------------- *)
+(* The next few theorems explore the properties of {INR i | i ∈ count n},    *)
+(* which can equivalently be described as {INR i | i < n}                     *)
+(* -------------------------------------------------------------------------- *)
+
+(* -------------------------------------------------------------------------- *)
+(* Fundamental inductive method used to produce a set of this form. This      *)
+(* allows us to work by induction on this set.                                *)
+(* -------------------------------------------------------------------------- *)
+Theorem INR_COMP_SUC:
+  ∀n : num.
+    {INR i | i < SUC n} = (INR n) INSERT {INR i | i < n}
+Proof
+  rpt strip_tac
+  >> irule (iffRL EXTENSION)
+  >> rpt strip_tac
+  >> Cases_on ‘x’ >> gvs[]
+QED
+
+(* -------------------------------------------------------------------------- *)
+(* In order to associate a finite cardinality with this set, we first need to *)
+(* know that it's finite.                                                     *)
+(* -------------------------------------------------------------------------- *)
+Theorem FINITE_INR_COMP[simp]:
+  ∀n : num.
+    FINITE {INR i | i < n}
+Proof
+  rpt strip_tac
+  >> Induct_on ‘n’ >> gvs[]
+  >> gvs[INR_COMP_SUC]
+QED
+
+(* -------------------------------------------------------------------------- *)
+(* Useful for simplification in fg_add_variable_node_wf                       *)
+(* -------------------------------------------------------------------------- *)
+Theorem CARD_INR_COMP[simp]:
+  ∀n.
+    CARD {INR i | i < n} = n
+Proof
+  rpt strip_tac >> gvs[]
+  >> Induct_on ‘n’ >> gvs[]
+  >> gvs[INR_COMP_SUC]
+QED
+
+(* -------------------------------------------------------------------------- *)
+(* Proof that after adding a variable node, the resulting factor graph will   *)
+(* be well-formed.                                                            *)
+(* -------------------------------------------------------------------------- *)
+Theorem fg_add_variable_node_wf[simp]:
+  ∀fg.
+    wffactor_graph fg ⇒
+    wffactor_graph (fg_add_variable_node fg)
+Proof
+  rpt strip_tac
+  >> gvs[wffactor_graph_def, fg_add_variable_node_def]
+  >- (qexists ‘SUC n’ >> gvs[INR_COMP_SUC])
+  >- (conj_tac
+      >- (Cases_on ‘n’ >> gvs[]
+          >> disj2_tac
+          >> gvs[gen_bipartite_def]
+          >> gvs[INR_COMP_SUC]
+          >> conj_tac
+          >- (gvs[UNION_DEF, INSERT_DEF]
+              >> irule (iffRL EXTENSION)
+              >> rpt strip_tac >> Cases_on ‘x’ >> gvs[]
+             )
+          >> rpt strip_tac
+          >> ‘F’ suffices_by gvs[] (* We cannot have any two edges in the orig *)
+
+                                Cases_on ‘{INR i | i < n} = ∅’ >> gvs[]
+QED
+
+(* -------------------------------------------------------------------------- *)
+(* Add a function node to the factor graph.                                    *)
+(*                                                                            *)
+(* Input:                                                                     *)
+(* - fg, the factor graph                                                     *)
+(* - f, the function to be added.                                             *)
+(*                                                                            *)
+(* Output:                                                                    *)
+(* - the factor graph with the new function node. The edges to other variable *)
+(* ts label will be the next  *)
+(*                                                                            *)
+(*                                                                            *)
+(*                                                                            *)
+(*   unused label.                                                            *)
+(* -------------------------------------------------------------------------- *)
+Definition fg_add_function_node_def:
+  fg_add_function_node fg f =
+  let
+    new_node = (INR (CARD (nodes fg.underlying_graph)))
+  in
+    fg with
+       <|
+         underlying_graph := fsgAddNode new_node fg.underlying_graph;
+         function_nodes := new_node INSERT fg.variable_nodes;
+         function_map := λfunction_label.
+                           if function_label = new_node
+                           then
+                             f
+                           else
+                             fg.function_map function_label
+       |>
+End
+
+(* -------------------------------------------------------------------------- *)
+(* Adding a function node to a factor graph maintains well-formedness         *)
+(* -------------------------------------------------------------------------- *)
+Theorem fg_add_function_node_wf[simp]:
+  ∀fg.
+    wffactor_graph fg ⇒
+    wffactor_graph (fg_add_variable_node fg)
+Proof
+  rpt strip_tac
+  >> gvs[wffactor_graph_def, fg_add_variable_node_def]
+QED
+
+(* -------------------------------------------------------------------------- *)
+(* Prove that two elements in a two-element set can be swapped                *)
+(* -------------------------------------------------------------------------- *)
+Theorem set_two_element_sym:
+  ∀n1 n2.
+    {n1; n2} = {n2; n1}
+Proof
+  rpt strip_tac
+  >> gvs[INSERT_DEF]
+  >> irule (iffRL EXTENSION)
+  >> rpt strip_tac
+  >> gvs[]
+  >> metis_tac[]
+QED
+
+(* -------------------------------------------------------------------------- *)
+(* Prove that adding an edge between two elements is the same regardless of   *)
+(* which order the two elements are provided in                               *)
+(* -------------------------------------------------------------------------- *)
+Theorem fg_add_edge_sym:
+  ∀fg n1 n2.
+    fg_add_edge fg n1 n2 = fg_add_edge fg n2 n1
+Proof
+  rpt strip_tac
+  >> gvs[fg_add_edge_def]
+  >> rw[]
+  >> Cases_on ‘n1 ∈ fg.variable_nodes’ >> Cases_on ‘n2 ∈ fg.variable_nodes’ >> Cases_on ‘n1 ∈ fg.function_nodes’ >> Cases_on ‘n2 ∈ fg.function_nodes’ >> gvs[]
+  >> gvs[set_two_element_sym]
+QED
+
+Theorem fg_add_edge_wf_spec:
+  ∀fg n1 n2.
+    (n1 ∈ fg.variable_nodes ∧ n2 ∈ fg.function_nodes) ⇒
+    wffactor_graph (fg_add_edge fg n1 n2)
+Proof
+  rpt strip_tac
+  >> gvs[wffactor_graph_def, fg_add_edge_def]
+  >> 
+QED
+
+Theorem fg_add_edge_wf:
+  ∀fg n1 n2.
+    ((n1 ∈ fg.variable_nodes ∧ n2 ∈ fg.function_nodes) ∨
+     (n1 ∈ fg.function_nodes ∧ n2 ∈ fg.variable_nodes)) ⇒
+    wffactor_graph (fg_add_edge fg n1 n2)
+Proof
+  rw[]
+  >> metis_tac[fg_add_edge_wf_spec, fg_add_edge_sym]
+QED
+
+(* -------------------------------------------------------------------------- *)
+(* Adds several variable and function nodes. This is intended to be much      *)
+(* easier to use than manually calling fg_add_variable_node and               *)
+(* fg_add_function_node repeatedly.                                            *)
+(*                                                                            *)
+(* Input:                                                                     *)
+(* - fg, the factor graph to add the nodes to.                                *)
+(* - nt::nts (aka. node types), a list of booleans, where the ith element is  *)
+(*   T if we need to add a function node and F if we need to add a variable   *)
+(*   node.                                                                    *)
+(* -------------------------------------------------------------------------- *)
+Theorem fg_add_variable_and_function_nodes:
+  fg_add_variable_and_function_nodes fg [] = fg ∧
+  fg_add_variable_and_function_nodes fg nt::nts =
+  let
+    recursive_call = fg_add_variable_and_function_nodes fg nts
+  in
+    if nt
+    then
+      fg_add_function_node      
+    else
+Proof
+QED
+
 
 (* -------------------------------------------------------------------------- *)
 (* Example 2.2 from Modern Coding Theory:                                     *)
@@ -184,6 +406,7 @@ End
 (* The following example factor graph is based on Example 2.2.                *)
 (* -------------------------------------------------------------------------- *)
 Definition fg_example_factor_graph_def:
+  fg_example_factor_graph = fg_add_variable_node ∘ fg_add_variable_node ∘ fg_add_function_node ∘ fg_add_variable_node fg_empty
 End
 
 Definition fg_example_functions_def:
